thys/POPLmark/Pattern.thy
@@ -28,201 +28,18 @@ fun PPTVars where
 lemma finite_PPVars: "finite (PPVars P)"
   by (induct P) auto
 
-definition nonrep_prepat :: "('tv::var, 'v) prepat \<Rightarrow> bool" where
-  "nonrep_prepat P = (\<forall>Q :: ('tv, 'v) prepat. rel_prepat top P Q \<longrightarrow> (\<exists>f. Q = map_prepat f P))"
-
-lemma nonrep_prepat_PPVar[simp]: "nonrep_prepat (PPVar x T)"
-  unfolding nonrep_prepat_def
+lemma ex_nonrep_prepat: "\<exists>(x :: ('a::var, 'b) prepat). \<forall>(Q :: ('a::var, 'b) prepat). rel_prepat top x Q \<longrightarrow> (\<exists>f. Q = map_prepat f x)"
+  apply (rule exI[of _ "PPVar undefined undefined"])
   apply safe
   subgoal for Q
     by (cases Q; auto)
   done
 
-lemma PVars_bd: "|PPVars (x :: ('tv::var, 'v::var) prepat)| <o |UNIV :: 'v::var set|"
-  by (rule ordLess_ordLeq_trans[OF prepat.set_bd]) (simp add: typ_pre.var_large)
-
-lemma values_lfupdate: "values (lfupdate X y x) \<subseteq> insert x (values X)"
-  including lfset.lifting
-  by transfer auto
-
-lemma map_lfset_lfupdate: "map_lfset id f (lfupdate X y x) = lfupdate (map_lfset id f X) y (f x)"
-  including lfset.lifting
-  by transfer (auto 0 4 simp: image_iff map_prod_def split_beta)
-
-lemma lfupdate_idle: "(y, Q) \<in>\<in> X \<Longrightarrow> X\<lbrace>y := Q\<rbrace> = X"
-  including lfset.lifting
-  by transfer (auto simp: nonrep_lfset_alt)
-
-lemma lfin_lfupdate: "(x, Q) \<in>\<in> X\<lbrace>y := T\<rbrace> \<longleftrightarrow> (if x = y then Q = T else (x, Q) \<in>\<in> X)"
-  including lfset.lifting
-  by transfer auto
-
-lemma map_prepat_idleD: "map_prepat f P = P \<Longrightarrow> z \<in> PPVars P \<Longrightarrow> f z = z"
-  apply (induct P)
-   apply auto
-  by (metis lfin_label_inject lfin_map_lfset values_lfin)
-
-lemma map_prepat_swapD: "map_prepat f Q = map_prepat (id(z := z', z' := z)) Q \<Longrightarrow> z \<in> PPVars Q \<Longrightarrow> f z = z'"
-  apply (induct Q)
-   apply auto
-  by (metis (no_types, opaque_lifting) lfin_label_inject lfin_map_lfset values_lfin)
-
-lemma nonrep_prepat_PRecD1: "nonrep_prepat (PPRec X :: ('tv::var, 'v::var) prepat) \<Longrightarrow> (x, P) \<in>\<in> X \<Longrightarrow>
-  nonrep_prepat P"
-  unfolding nonrep_prepat_def
-proof safe
-  fix Q :: "('tv, 'v) prepat"
-  assume shape: "\<forall>Q. rel_prepat top (PPRec X) (Q::('tv, 'v) prepat) \<longrightarrow> (\<exists>f. Q = map_prepat f (PPRec X))"
-    and PQ: "(x, P) \<in>\<in> X" "rel_prepat top P Q"
-  then have "rel_prepat top (PPRec X) (PPRec (X\<lbrace>x := Q\<rbrace>))"
-    by (auto simp: lfset.in_rel[of id, simplified, unfolded lfset.map_id]
-      map_lfset_lfupdate lfset.set_map lfset.map_comp o_def lfset.map_ident prepat.rel_refl lfupdate_idle
-      dest!: set_mp[OF values_lfupdate]
-      intro!: exI[of _ "lfupdate (map_lfset id (\<lambda>P. (P, P)) X) x (P, Q)"]) []
-  from shape[rule_format, OF this] show "\<exists>f. Q = map_prepat f P"
-  proof (elim ex_reg[rotated], intro allI impI)
-    fix f :: "'v \<Rightarrow> 'v"
-    assume "PPRec (X\<lbrace>x := Q\<rbrace>) =  map_prepat f (PPRec X)"
-    with PQ show "Q = map_prepat f P"
-      by (metis (mono_tags, lifting) lfin_lfupdate lfin_map_lfset prepat.inject(2)
-          prepat.simps(10))
-  qed
-qed
-
-lemma nonrep_prepat_PRecD2: "nonrep_prepat (PPRec X :: ('tv::var, 'v::var) prepat) \<Longrightarrow>
-  (\<forall>x y P Q. x \<noteq> y \<longrightarrow> (x, P) \<in>\<in> X \<longrightarrow> (y, Q) \<in>\<in> X \<longrightarrow> PPVars P \<inter> PPVars Q = {})"
-proof (unfold nonrep_prepat_def, safe, goal_cases LR)
-  case (LR x y P Q z)
-  obtain z' where "z' \<notin> PPVars (PPRec X)"
-    using MRBNF_FP.exists_fresh[OF PVars_bd] by blast
-  with LR(4) have "rel_prepat top (PPRec X) (PPRec (lfupdate X y (map_prepat (id(z := z', z' := z)) Q)))"
-    by (auto simp: lfset.in_rel[of id, simplified, unfolded lfset.map_id]
-      map_lfset_lfupdate lfset.map_comp o_def lfset.map_ident
-      prepat.rel_map prepat.rel_refl lfset.set_map lfupdate_idle
-      dest!: set_mp[OF values_lfupdate]
-      intro!: exI[of _ "lfupdate (map_lfset id (\<lambda>P. (P, P)) X) y (Q, map_prepat (id(z := z', z' := z)) Q)"])
-  with LR(1) obtain f where "map_prepat f (PPRec X) = PPRec (lfupdate X y (map_prepat (id(z := z', z' := z)) Q))"
-    by metis
-  then have *: "map_lfset id (map_prepat f) X = X\<lbrace>y := map_prepat (id(z := z', z' := z)) Q\<rbrace>"
-    by (auto dest!: arg_cong[where f=PPVars])
-  then have "map_prepat f P = P"
-    using LR(2) lfin_map_lfset[THEN iffD2, OF exI, OF conjI, OF _ LR(3), of "map_prepat f P" "map_prepat f"]
-    by (auto simp: lfin_lfupdate lfin_label_inject LR(3))
-  then have "f z = z"
-    using LR(5) map_prepat_idleD by metis
-  moreover from * have "map_prepat f Q = map_prepat (id(z := z', z' := z)) Q"
-    using lfin_map_lfset[THEN iffD2, OF exI, OF conjI, OF _ LR(4), of "map_prepat f Q" "map_prepat f"]
-    by (auto simp: lfin_lfupdate)
-  then have "f z = z'"
-    using LR(6) map_prepat_swapD by metis
-  ultimately show ?case
-    by (metis LR(3,5) \<open>z' \<notin> PPVars (PPRec X)\<close> lfin_values prepat.set_intros(2))
-qed
-
-lemma lfset_eq_iff: "X = Y \<longleftrightarrow> (\<forall>x P. (x, P) \<in>\<in> X \<longleftrightarrow> (x, P) \<in>\<in> Y)"
-  including lfset.lifting
-  by transfer auto
-
-lemma nonrep_prepat_PRecI:
-  assumes
-    "(\<forall>x P. (x, P) \<in>\<in> X \<longrightarrow> nonrep_prepat P)"
-    "(\<forall>x y P Q. x \<noteq> y \<longrightarrow> (x, P) \<in>\<in> X \<longrightarrow> (y, Q) \<in>\<in> X \<longrightarrow> PPVars P \<inter> PPVars Q = {})"
-  shows "nonrep_prepat (PPRec X :: ('tv::var, 'v::var) prepat)"
-  using assms
-  unfolding nonrep_prepat_def
-proof (safe, goal_cases RL)
-  case (RL QQ)
-  then obtain Y where "QQ = PPRec Y"
-    by (cases QQ; simp)
-  with RL(3) have *: "rel_lfset id (rel_prepat top) X Y" by auto
-  { fix x P
-    assume xP: "(x, P) \<in>\<in> X"
-    with * obtain Q where "(x, Q) \<in>\<in> Y" "rel_prepat top P Q"
-      including lfset.lifting
-      by (atomize_elim, transfer) (force simp: rel_fset_alt)
-    moreover
-    from assms(1) xP \<open>rel_prepat top P Q\<close> obtain f where "map_prepat f P = Q"
-      unfolding nonrep_prepat_def by blast
-    then obtain g where "supp g \<subseteq> PPVars P" "map_prepat g P = Q"
-      by (atomize_elim, intro exI[of _ "\<lambda>x. if x \<in> PPVars P then f x else x"])
-        (auto simp: supp_def intro: prepat.map_cong)
-    ultimately have "\<exists>f. (x, map_prepat f P) \<in>\<in> Y \<and> supp f \<subseteq> PPVars P"
-      by auto
-  } note pick_ex = this
-  define pick where "pick = (\<lambda>x (P :: ('tv::var, 'v::var) prepat). SOME f. (x, map_prepat f P) \<in>\<in> Y \<and> supp f \<subseteq> PPVars P)"
-  have pick: "(x, map_prepat (pick x P) P) \<in>\<in> Y" "supp (pick x P) \<subseteq> PPVars P" if "(x, P) \<in>\<in> X" for x P
-    using someI_ex[OF pick_ex[OF that]] unfolding pick_def
-    by (auto simp: Eps_case_prod)
-  define pick_part where "pick_part = (\<lambda>z. THE (x, P). (x, P) \<in>\<in> X \<and> z \<in> PPVars P)"
-  have pick_part: "pick_part z \<in>\<in> X \<and> z \<in> PPVars (snd (pick_part z))" if "\<exists>x P. (x, P) \<in>\<in> X \<and> z \<in> PPVars P" for z
-    using that assms(2) unfolding pick_part_def
-    apply -
-    apply (rule the1I2)
-     apply auto
-     apply blast
-    by (metis Int_emptyD lfin_label_inject)
-  define pick1 where "pick1 = (\<lambda>z. if \<exists>x P. (x, P) \<in>\<in> X \<and> z \<in> PPVars P then case_prod pick (pick_part z) z else z)"
-  show ?case
-    unfolding \<open>QQ = PPRec Y\<close>
-    apply (auto intro!: exI[of _ pick1] simp: pick1_def lfset_eq_iff lfin_map_lfset)
-    subgoal for x P
-      apply (subgoal_tac "\<exists>P'. (x, P') \<in>\<in> X \<and> rel_prepat top P' P")
-       apply auto
-       apply (frule pick)
-      subgoal for P'
-        apply (rule exI[of _ P'])
-        apply auto
-        apply (rule sym)
-        apply (rule trans[OF prepat.map_cong[OF refl]])
-         apply (rule if_P)
-         apply (auto simp: split_beta)
-        apply (rule trans[OF prepat.map_cong[OF refl], of _ _ "pick x P'"])
-        apply (metis Int_emptyD assms(2) lfin_label_inject pick_part surjective_pairing)
-        apply (simp add: lfin_label_inject)
-        done
-      subgoal
-        using *
-        including lfset.lifting
-        by transfer (force simp: rel_fset_alt)
-      done
-    subgoal for x P
-      apply (frule pick)
-      using
-        \<open>\<And>x P. (x, P) \<in>\<in> Y \<Longrightarrow> \<exists>c. P = map_prepat (\<lambda>z. if \<exists>x P. (x, P) \<in>\<in> X \<and> z \<in> PPVars P then (case pick_part z of (x, xa) \<Rightarrow> pick x xa) z else z) c \<and> (x, c) \<in>\<in> X\<close>
-        lfin_label_inject by fastforce
-    done
-qed
-
-definition "nonrep_PPRec X = (\<forall>x y P Q. x \<noteq> y \<longrightarrow> (x, P) \<in>\<in> X \<longrightarrow> (y, Q) \<in>\<in> X \<longrightarrow> PPVars P \<inter> PPVars Q = {})"
-
-lemma nonrep_PPRec_lfemtpy[simp]: "nonrep_PPRec lfempty"
-  unfolding nonrep_PPRec_def by auto
-
-lemma nonrep_prepat_PRec[simp]: "nonrep_prepat (PPRec X :: ('tv::var, 'v::var) prepat) \<longleftrightarrow>
-  ((\<forall>x P. (x, P) \<in>\<in> X \<longrightarrow> nonrep_prepat P) \<and>
-  nonrep_PPRec X)"
-  unfolding nonrep_PPRec_def
-  using nonrep_prepat_PRecI[of X] nonrep_prepat_PRecD1[of X] nonrep_prepat_PRecD2[of X] by blast
-
-lemma rel_prepat_alt: "(\<exists>R. rel_prepat R x x') = rel_prepat top x x'"
-  apply (rule iffI)
-   apply (erule exE)
-   apply (rule prepat.rel_mono_strong)
-    apply (assumption)
-   apply (unfold top_apply top_bool_def) []
-   apply (rule TrueI)
-  apply (rule exI)
-  apply (assumption)
-  done
-
-lemma ex_nonrep_prepat: "\<exists>x. nonrep_prepat x"
-  apply (unfold nonrep_prepat_def)
-  by (auto intro!: exI[of _ "PPVar undefined undefined"] simp add: nonrep_prepat_def[symmetric])
-
 lemma map_vvsubst_equiv: "map_prepat f x = vvsubst_prepat id f x"
   apply (induction x)
    apply (auto simp add: lfset.map_cong_id typ.map_ident)
   done
+
 
 mrbnf "('tv :: var, 'v) prepat"
   map: vvsubst_prepat
@@ -230,7 +47,7 @@ mrbnf "('tv :: var, 'v) prepat"
     free: PPTVars
     live: PPVars
   bd: "natLeq"
-  wits: "PPRec lfempty"
+  (*wits: "PPRec lfempty"*)
   rel: "rel_prepat"
   subgoal
     apply (rule prepat.map_id0[unfolded map_vvsubst_equiv])
@@ -310,10 +127,11 @@ mrbnf "('tv :: var, 'v) prepat"
         done
       done
     done
-  subgoal by (auto)
   done
 
-linearize_mrbnf ('tv::var, 'v) pat' = "('tv::var, 'v) prepat" [wits:"(PPRec lfempty) :: ('tv::var, 'v) prepat"] on 'v
+declare [[ML_print_depth=1000]]
+
+linearize_mrbnf ('tv::var, 'v::var) pat = "('tv::var, 'v::var) prepat" [wits:"(PPRec lfempty) :: ('tv::var, 'v::var) prepat"] on 'v
 subgoal for R x y
     apply (unfold P.Pattern.P.prepat.in_rel mem_Collect_eq map_vvsubst_equiv)
     apply (rule iffI)
@@ -353,24 +171,207 @@ subgoal for R x y
     qed
     done
   subgoal
-    apply (rule ex_nonrep_prepat[unfolded nonrep_prepat_def map_vvsubst_equiv])
+    apply (rule ex_nonrep_prepat[unfolded map_vvsubst_equiv])
     done
-  apply auto?
+  apply (unfold prepat.in_rel[OF supp_id_bound, unfolded prepat.map_id])
+  apply (intro allI impI exI[of _ id])
+  apply (unfold prepat.map_id)
+  apply (auto)
+  apply (rule trans[OF sym, rotated])
+   apply assumption
+  apply (rule prepat.map_cong; (rule supp_id_bound refl)?)
+  apply (drule arg_cong[where f=PPVars])
+  apply (simp add: prepat.set_map)
   done
+
+lemma nonrep_prepat_def_alt: "nonrep_prepat (x :: ('tv::var, 'v::var) prepat) 
+  \<equiv> \<forall>(Q :: ('tv::var, 'v::var) prepat). rel_prepat top x Q \<longrightarrow> (\<exists>f. Q = map_prepat f x)"
+  unfolding nonrep_prepat_def sameShape_prepat_def mr_rel_prepat_def map_vvsubst_equiv[THEN sym] P.Pattern.P.prepat.map_id
+  by simp
+
+lemma nonrep_prepat_PPVar[simp]: "nonrep_prepat (PPVar x T)"
+  unfolding nonrep_prepat_def_alt
+  apply safe
+  subgoal for Q
+    by (cases Q; auto)
+  done
+
+lemma PVars_bd: "|PPVars (x :: ('tv::var, 'v::var) prepat)| <o |UNIV :: 'v::var set|"
+  by (rule ordLess_ordLeq_trans[OF prepat.set_bd(2)]) (simp add: typ_pre.var_large)
+
+lemma values_lfupdate: "values (lfupdate X y x) \<subseteq> insert x (values X)"
+  including lfset.lifting
+  by transfer auto
+
+lemma map_lfset_lfupdate: "map_lfset id f (lfupdate X y x) = lfupdate (map_lfset id f X) y (f x)"
+  including lfset.lifting
+  by transfer (auto 0 4 simp: image_iff map_prod_def split_beta)
+
+lemma lfupdate_idle: "(y, Q) \<in>\<in> X \<Longrightarrow> X\<lbrace>y := Q\<rbrace> = X"
+  including lfset.lifting
+  by transfer (auto simp: nonrep_lfset_alt)
+
+lemma lfin_lfupdate: "(x, Q) \<in>\<in> X\<lbrace>y := T\<rbrace> \<longleftrightarrow> (if x = y then Q = T else (x, Q) \<in>\<in> X)"
+  including lfset.lifting
+  by transfer auto
+
+lemma map_prepat_idleD: "map_prepat f P = P \<Longrightarrow> z \<in> PPVars P \<Longrightarrow> f z = z"
+  apply (induct P)
+   apply auto
+  by (metis lfin_label_inject lfin_map_lfset values_lfin)
+
+lemma map_prepat_swapD: "map_prepat f Q = map_prepat (id(z := z', z' := z)) Q \<Longrightarrow> z \<in> PPVars Q \<Longrightarrow> f z = z'"
+  apply (induct Q)
+   apply auto
+  by (metis (no_types, opaque_lifting) lfin_label_inject lfin_map_lfset values_lfin)
+
+lemma nonrep_prepat_PRecD1: "nonrep_prepat (PPRec X :: ('tv::var, 'v::var) prepat) \<Longrightarrow> (x, P) \<in>\<in> X \<Longrightarrow>
+  nonrep_prepat P"
+  unfolding nonrep_prepat_def_alt
+proof safe
+  fix Q :: "('tv, 'v) prepat"
+  assume shape: "\<forall>Q. rel_prepat top (PPRec X) (Q::('tv, 'v) prepat) \<longrightarrow> (\<exists>f. Q = map_prepat f (PPRec X))"
+    and PQ: "(x, P) \<in>\<in> X" "rel_prepat top P Q"
+  then have "rel_prepat top (PPRec X) (PPRec (X\<lbrace>x := Q\<rbrace>))"
+    by (auto simp: lfset.in_rel[of id, simplified, unfolded lfset.map_id]
+      map_lfset_lfupdate lfset.set_map lfset.map_comp o_def lfset.map_ident prepat.rel_refl lfupdate_idle
+      dest!: set_mp[OF values_lfupdate]
+      intro!: exI[of _ "lfupdate (map_lfset id (\<lambda>P. (P, P)) X) x (P, Q)"]) []
+  from shape[rule_format, OF this] show "\<exists>f. Q = map_prepat f P"
+  proof (elim ex_reg[rotated], intro allI impI)
+    fix f :: "'v \<Rightarrow> 'v"
+    assume "PPRec (X\<lbrace>x := Q\<rbrace>) =  map_prepat f (PPRec X)"
+    with PQ show "Q = map_prepat f P"
+      by (metis (mono_tags, lifting) lfin_lfupdate lfin_map_lfset prepat.inject(2)
+          prepat.simps(10))
+  qed
+qed
+
+lemma nonrep_prepat_PRecD2: "nonrep_prepat (PPRec X :: ('tv::var, 'v::var) prepat) \<Longrightarrow>
+  (\<forall>x y P Q. x \<noteq> y \<longrightarrow> (x, P) \<in>\<in> X \<longrightarrow> (y, Q) \<in>\<in> X \<longrightarrow> PPVars P \<inter> PPVars Q = {})"
+  unfolding nonrep_prepat_def_alt
+proof (safe, goal_cases LR)
+  case (LR x y P Q z)
+  obtain z' where "z' \<notin> PPVars (PPRec X)"
+    using MRBNF_FP.exists_fresh[OF PVars_bd] by blast
+  with LR(4) have "rel_prepat top (PPRec X) (PPRec (lfupdate X y (map_prepat (id(z := z', z' := z)) Q)))"
+    by (auto simp: lfset.in_rel[of id, simplified, unfolded lfset.map_id]
+      map_lfset_lfupdate lfset.map_comp o_def lfset.map_ident
+      P.Pattern.P.prepat.rel_map prepat.rel_refl lfset.set_map lfupdate_idle
+      dest!: set_mp[OF values_lfupdate]
+      intro!: exI[of _ "lfupdate (map_lfset id (\<lambda>P. (P, P)) X) y (Q, map_prepat (id(z := z', z' := z)) Q)"])
+  with LR(1) obtain f where "map_prepat f (PPRec X) = PPRec (lfupdate X y (map_prepat (id(z := z', z' := z)) Q))"
+    by metis
+  then have *: "map_lfset id (map_prepat f) X = X\<lbrace>y := map_prepat (id(z := z', z' := z)) Q\<rbrace>"
+    by (auto dest!: arg_cong[where f=PPVars])
+  then have "map_prepat f P = P"
+    using LR(2) lfin_map_lfset[THEN iffD2, OF exI, OF conjI, OF _ LR(3), of "map_prepat f P" "map_prepat f"]
+    by (auto simp: lfin_lfupdate lfin_label_inject LR(3))
+  then have "f z = z"
+    using LR(5) map_prepat_idleD by metis
+  moreover from * have "map_prepat f Q = map_prepat (id(z := z', z' := z)) Q"
+    using lfin_map_lfset[THEN iffD2, OF exI, OF conjI, OF _ LR(4), of "map_prepat f Q" "map_prepat f"]
+    by (auto simp: lfin_lfupdate)
+  then have "f z = z'"
+    using LR(6) map_prepat_swapD by metis
+  ultimately show ?case
+    by (metis LR(3,5) \<open>z' \<notin> PPVars (PPRec X)\<close> lfin_values prepat.set_intros(2))
+qed
+
+lemma lfset_eq_iff: "X = Y \<longleftrightarrow> (\<forall>x P. (x, P) \<in>\<in> X \<longleftrightarrow> (x, P) \<in>\<in> Y)"
+  including lfset.lifting
+  by transfer auto
+
+lemma nonrep_prepat_PRecI:
+  assumes
+    "(\<forall>x P. (x, P) \<in>\<in> X \<longrightarrow> nonrep_prepat P)"
+    "(\<forall>x y P Q. x \<noteq> y \<longrightarrow> (x, P) \<in>\<in> X \<longrightarrow> (y, Q) \<in>\<in> X \<longrightarrow> PPVars P \<inter> PPVars Q = {})"
+  shows "nonrep_prepat (PPRec X :: ('tv::var, 'v::var) prepat)"
+  using assms
+  unfolding nonrep_prepat_def_alt
+proof (safe, goal_cases RL)
+  case (RL QQ)
+  then obtain Y where "QQ = PPRec Y"
+    by (cases QQ; simp)
+  with RL(3) have *: "rel_lfset id (rel_prepat top) X Y" by auto
+  { fix x P
+    assume xP: "(x, P) \<in>\<in> X"
+    with * obtain Q where "(x, Q) \<in>\<in> Y" "rel_prepat top P Q"
+      including lfset.lifting
+      by (atomize_elim, transfer) (force simp: rel_fset_alt)
+    moreover
+    from assms(1) xP \<open>rel_prepat top P Q\<close> obtain f where "map_prepat f P = Q"
+      unfolding nonrep_prepat_def_alt
+      by blast
+    then obtain g where "supp g \<subseteq> PPVars P" "map_prepat g P = Q"
+      by (atomize_elim, intro exI[of _ "\<lambda>x. if x \<in> PPVars P then f x else x"])
+        (auto simp: supp_def 
+          intro: prepat.map_cong[OF supp_id_bound supp_id_bound, unfolded map_vvsubst_equiv[THEN sym] id_apply])
+    ultimately have "\<exists>f. (x, map_prepat f P) \<in>\<in> Y \<and> supp f \<subseteq> PPVars P"
+      by auto
+  } note pick_ex = this
+  define pick where "pick = (\<lambda>x (P :: ('tv::var, 'v::var) prepat). SOME f. (x, map_prepat f P) \<in>\<in> Y \<and> supp f \<subseteq> PPVars P)"
+  have pick: "(x, map_prepat (pick x P) P) \<in>\<in> Y" "supp (pick x P) \<subseteq> PPVars P" if "(x, P) \<in>\<in> X" for x P
+    using someI_ex[OF pick_ex[OF that]] unfolding pick_def
+    by (auto simp: Eps_case_prod)
+  define pick_part where "pick_part = (\<lambda>z. THE (x, P). (x, P) \<in>\<in> X \<and> z \<in> PPVars P)"
+  have pick_part: "pick_part z \<in>\<in> X \<and> z \<in> PPVars (snd (pick_part z))" if "\<exists>x P. (x, P) \<in>\<in> X \<and> z \<in> PPVars P" for z
+    using that assms(2) unfolding pick_part_def
+    apply -
+    apply (rule the1I2)
+     apply auto
+     apply blast
+    by (metis Int_emptyD lfin_label_inject)
+  define pick1 where "pick1 = (\<lambda>z. if \<exists>x P. (x, P) \<in>\<in> X \<and> z \<in> PPVars P then case_prod pick (pick_part z) z else z)"
+  show ?case
+    unfolding \<open>QQ = PPRec Y\<close>
+    apply (auto intro!: exI[of _ pick1] simp: pick1_def lfset_eq_iff lfin_map_lfset)
+    subgoal for x P
+      apply (subgoal_tac "\<exists>P'. (x, P') \<in>\<in> X \<and> rel_prepat top P' P")
+       apply auto
+       apply (frule pick)
+      subgoal for P'
+        apply (rule exI[of _ P'])
+        apply auto
+        apply (rule sym)
+        (*\<lbrakk>\<And>z. z \<in> PPVars ?x1 \<Longrightarrow> ?f1 z = ?g1 z; map_prepat ?g1 ?x1 = ?t\<rbrakk> \<Longrightarrow> map_prepat ?f1 ?x1 = ?t*)
+        apply (rule trans[OF prepat.map_cong[OF supp_id_bound supp_id_bound refl, unfolded map_vvsubst_equiv[THEN sym] id_apply]])
+        apply (rule refl)
+         apply (rule if_P)
+         apply (auto simp: split_beta)
+        apply (rule trans[OF prepat.map_cong[OF supp_id_bound supp_id_bound refl, unfolded map_vvsubst_equiv[THEN sym] id_apply], of _ _ "pick x P'"])
+        apply (rule refl)
+        apply (metis Int_emptyD assms(2) lfin_label_inject pick_part surjective_pairing)
+        apply (simp add: lfin_label_inject)
+        done
+      subgoal
+        using *
+        including lfset.lifting
+        by transfer (force simp: rel_fset_alt)
+      done
+    subgoal for x P
+      apply (frule pick)
+      using
+        \<open>\<And>x P. (x, P) \<in>\<in> Y \<Longrightarrow> \<exists>c. P = map_prepat (\<lambda>z. if \<exists>x P. (x, P) \<in>\<in> X \<and> z \<in> PPVars P then (case pick_part z of (x, xa) \<Rightarrow> pick x xa) z else z) c \<and> (x, c) \<in>\<in> X\<close>
+        lfin_label_inject by fastforce
+    done
+qed
+
+definition "nonrep_PPRec X = (\<forall>x y P Q. x \<noteq> y \<longrightarrow> (x, P) \<in>\<in> X \<longrightarrow> (y, Q) \<in>\<in> X \<longrightarrow> PPVars P \<inter> PPVars Q = {})"
+
+lemma nonrep_PPRec_lfemtpy[simp]: "nonrep_PPRec lfempty"
+  unfolding nonrep_PPRec_def by auto
+
+lemma nonrep_prepat_PRec[simp]: "nonrep_prepat (PPRec X :: ('tv::var, 'v::var) prepat) \<longleftrightarrow>
+  ((\<forall>x P. (x, P) \<in>\<in> X \<longrightarrow> nonrep_prepat P) \<and>
+  nonrep_PPRec X)"
+  unfolding nonrep_PPRec_def
+  using nonrep_prepat_PRecI[of X] nonrep_prepat_PRecD1[of X] nonrep_prepat_PRecD2[of X] by blast
 
 
 setup_lifting type_definition_pat
 
-thm prepat.map_id
-
-lemma nonrep_prepat_alt: "nonrep'_prepat x \<equiv> nonrep_prepat x"
-  apply (unfold nonrep'_prepat_def sameShape'_prepat_def nonrep_prepat_def rel_prepat_alt[symmetric] prepat.map_id
-      mr_rel_prepat_def map_vvsubst_equiv)
-  apply (assumption)
-  done
-
 lift_definition PVar :: "'v \<Rightarrow> 'tv typ \<Rightarrow> ('tv::var, 'v::var) pat" is PPVar
-  apply (unfold nonrep_prepat_alt)
   by (rule nonrep_prepat_PPVar)
 
 lemma PVar_inject[simp]: "PVar X T = PVar Y U \<longleftrightarrow> X = Y \<and> T = U"
@@ -383,9 +384,9 @@ lemma PRec_transfer[transfer_rule]: "rel_fun (rel_lfset id cr_pat) cr_pat (\<lam
   apply (auto simp: PRec_def rel_fun_def cr_pat_def lfset.map_comp Abs_pat_inverse
     lfset.in_rel[of id, simplified, unfolded lfset.map_id])
   apply (subst Abs_pat_inverse)
-     apply (auto simp: Abs_pat_inverse lfin_map_lfset Rep_pat Collect_prod_beta subset_eq nonrep_prepat_alt
+     apply (auto simp: Abs_pat_inverse lfin_map_lfset Rep_pat Collect_prod_beta subset_eq
        intro!: lfset.map_cong)
-  using Rep_pat[unfolded nonrep_prepat_alt] apply blast
+  using Rep_pat apply blast
   apply (simp_all add: lfset.map_cong_id)
   done
 (*
@@ -423,13 +424,22 @@ lemma PPTVars_tvsubst_prepat[simp]:
 lemma nonrep_prepat_vvsubst_prepat:
   "bij \<sigma> \<Longrightarrow> nonrep_prepat (P::('tv::var,'v::var) prepat) \<Longrightarrow> nonrep_prepat (vvsubst_prepat \<tau> \<sigma> P::('tv::var,'v::var) prepat)"
   apply (induct P)
-   apply (auto simp: lfin_map_lfset lfin_values nonrep_PPRec_def)
+
+(* 1. \<And>x1 x2a.
+       \<lbrakk>bij \<sigma>; nonrep_prepat (PPVar x1 x2a)\<rbrakk>
+       \<Longrightarrow> nonrep_prepat (vvsubst_prepat \<tau> \<sigma> (PPVar x1 x2a))
+ 2. \<And>x. \<lbrakk>\<And>xa. \<lbrakk>xa \<in> values x; bij \<sigma>; nonrep_prepat xa\<rbrakk>
+               \<Longrightarrow> nonrep_prepat (vvsubst_prepat \<tau> \<sigma> xa);
+          bij \<sigma>; nonrep_prepat (PPRec x)\<rbrakk>
+         \<Longrightarrow> nonrep_prepat (vvsubst_prepat \<tau> \<sigma> (PPRec x))*)
+  apply (simp add: lfin_map_lfset lfin_values nonrep_PPRec_def)
+   apply (auto simp: lfin_map_lfset lfin_values nonrep_PPRec_def )
   apply (metis Int_emptyD bij_implies_inject)
   done
 
 lift_definition vvsubst_pat :: "('tv \<Rightarrow> 'tv) \<Rightarrow> ('v \<Rightarrow> 'v) \<Rightarrow> ('tv::var, 'v::var) pat \<Rightarrow> ('tv::var, 'v::var) pat" is
   "\<lambda>\<tau> \<sigma>. if bij \<sigma> then vvsubst_prepat \<tau> \<sigma> else id"
-  by (auto simp: nonrep_prepat_vvsubst_prepat nonrep_prepat_alt)
+  by (auto simp: nonrep_prepat_vvsubst_prepat)
 
 lemma nonrep_prepat_tvsubst_prepat:
   "bij \<sigma> \<Longrightarrow> nonrep_prepat (P::('tv::var,'v::var) prepat) \<Longrightarrow> nonrep_prepat (tvsubst_prepat \<tau> \<sigma> P::('tv::var,'v::var) prepat)"
@@ -440,7 +450,7 @@ lemma nonrep_prepat_tvsubst_prepat:
 
 lift_definition tvsubst_pat :: "('tv \<Rightarrow> 'tv typ) \<Rightarrow> ('v \<Rightarrow> 'v) \<Rightarrow> ('tv::var, 'v::var) pat \<Rightarrow> ('tv::var, 'v::var) pat" is
   "\<lambda>\<tau> \<sigma>. if bij \<sigma> then tvsubst_prepat \<tau> \<sigma> else id"
-  by (auto simp: nonrep_prepat_tvsubst_prepat nonrep_prepat_alt)
+  by (auto simp: nonrep_prepat_tvsubst_prepat)
 
 lift_definition PVars :: "('tv::var, 'v::var) pat \<Rightarrow> 'v set" is
   "PPVars" .
@@ -506,70 +516,9 @@ lemma vvsubst_pat_id[simp]: "vvsubst_pat id id P = P"
   apply transfer
   subgoal for P
     apply (induct P)
-     apply (force simp: typ.map_id values_lfin_iff nonrep_prepat_alt intro!: trans[OF lfset.map_cong_id lfset.map_id])+
+     apply (force simp: typ.map_id values_lfin_iff intro!: trans[OF lfset.map_cong_id lfset.map_id])+
     done
   done
-
-(*mrbnf "('tv :: var, 'v :: var) pat"
-  map: vvsubst_pat
-  sets:
-    free: PTVars
-    bound: PVars
-  bd: "natLeq"
-  rel: "(=)"
-  subgoal
-    apply (rule ext)
-    apply simp
-    done
-  subgoal for f1 f2 g1 g2
-    apply (rule ext)
-    apply (transfer fixing: f1 f2 g1 g2)
-    subgoal for P
-      apply (induct P)
-       apply (force simp: typ.map_comp lfset.map_comp values_lfin_iff nonrep_prepat_alt intro!: lfset.map_cong)+
-      done
-    done
-  subgoal for P f1 f2 g1 g2
-    apply (transfer fixing: f1 f2 g1 g2)
-    subgoal for P
-      apply (induct P)
-       apply (fastforce simp: values_lfin_iff Bex_def nonrep_prepat_alt intro!: typ.map_cong lfset.map_cong)+
-      done
-    done
-  subgoal for f g
-    apply (rule ext)
-    apply (transfer fixing: f g)
-    subgoal for P
-      apply (induct P)
-       apply (fastforce simp: typ.set_map lfset.set_map values_lfin_iff)+
-      done
-    done
-  subgoal for f g
-    apply (rule ext)
-    apply (transfer fixing: f g)
-    subgoal for P
-      apply (induct P)
-       apply (fastforce simp: typ.set_map lfset.set_map values_lfin_iff)+
-      done
-    done
-  subgoal by (simp add: infinite_regular_card_order_natLeq)
-  subgoal for P
-    apply transfer
-    subgoal for P
-    apply (induct P)
-       apply (force simp: typ.FVars_bd lfset.set_bd values_lfin_iff nonrep_prepat_alt intro!: stable_UNION[OF stable_natLeq])+
-      done
-    done
-  subgoal for P
-    apply transfer
-    subgoal for P
-    apply (induct P)
-       apply (force simp: typ.FVars_bd lfset.set_bd ID.set_bd values_lfin_iff nonrep_prepat_alt intro!: stable_UNION[OF stable_natLeq])+
-      done
-    done
-  subgoal by simp
-  subgoal by simp
-  done*)
 
 lemma vvsubst_pat_PVar[simp]:
   "bij g \<Longrightarrow> vvsubst_pat f g (PVar x T) = PVar (g x) (vvsubst_typ f T)"
@@ -591,9 +540,9 @@ lemma PRec_inject[simp]: "nonrep_PRec PP \<Longrightarrow> nonrep_PRec UU \<Long
   unfolding PRec_def
   apply (auto simp: nonrep_PRec_alt)
   apply (subst (asm) Abs_pat_inject)
-    apply (auto simp: Rep_pat_inject nonrep_prepat_alt elim!: lfset.inj_map_strong[rotated])
-  apply (metis Rep_pat nonrep_prepat_alt lfin_map_lfset mem_Collect_eq)
-  apply (metis Rep_pat nonrep_prepat_alt lfin_map_lfset mem_Collect_eq)
+    apply (auto simp: Rep_pat_inject elim!: lfset.inj_map_strong[rotated])
+  apply (metis Rep_pat lfin_map_lfset mem_Collect_eq)
+  apply (metis Rep_pat lfin_map_lfset mem_Collect_eq)
   done
 
 lemma vvsubst_pat_PRec[simp]:
@@ -601,18 +550,18 @@ lemma vvsubst_pat_PRec[simp]:
   unfolding PRec_def vvsubst_pat_def nonrep_PRec_alt
   apply (auto simp: lfset.map_comp o_def map_fun_def id_def[symmetric])
      apply (subst (1 2) Abs_pat_inverse)
-  using Rep_pat nonrep_prepat_vvsubst_prepat nonrep_prepat_alt apply blast
-    apply (auto simp: nonrep_prepat_alt) []
-      apply (metis Rep_pat lfin_map_lfset mem_Collect_eq nonrep_prepat_alt)
+  using Rep_pat nonrep_prepat_vvsubst_prepat apply blast
+  apply (auto) []
+      apply (metis Rep_pat lfin_map_lfset mem_Collect_eq)
      apply (subst Abs_pat_inject)
   apply (metis (mono_tags, lifting) Rep_pat lfin_map_lfset mem_Collect_eq nonrep_prepat_PRec
-      nonrep_prepat_vvsubst_prepat nonrep_prepat_alt)
+      nonrep_prepat_vvsubst_prepat)
   apply (smt (verit, best) Abs_pat_inverse Rep_pat lfin_map_lfset lfset.map_cong_id
-      mem_Collect_eq nonrep_prepat_PRec nonrep_prepat_vvsubst_prepat nonrep_prepat_alt)
+      mem_Collect_eq nonrep_prepat_PRec nonrep_prepat_vvsubst_prepat)
      apply (auto simp: lfset.map_comp intro!: lfset.map_cong) []
   apply (smt (z3) Abs_pat_inverse Rep_pat lfin_map_lfset mem_Collect_eq nonrep_PPRec_def
       nonrep_prepat_PRec nonrep_prepat_vvsubst_prepat
-      vvsubst_prepat.simps(2) nonrep_prepat_alt)
+      vvsubst_prepat.simps(2))
   done
 
 lemma tvsubst_pat_PRec[simp]:
@@ -620,35 +569,33 @@ lemma tvsubst_pat_PRec[simp]:
   unfolding PRec_def tvsubst_pat_def nonrep_PRec_alt
   apply (auto simp: lfset.map_comp o_def map_fun_def id_def[symmetric])
      apply (subst (1 2) Abs_pat_inverse)
-  using Rep_pat nonrep_prepat_tvsubst_prepat nonrep_prepat_alt apply blast
-  apply (auto simp: nonrep_prepat_alt) []
-      apply (metis Rep_pat lfin_map_lfset mem_Collect_eq nonrep_prepat_alt)
+  using Rep_pat nonrep_prepat_tvsubst_prepat apply blast
+  apply (auto) []
+      apply (metis Rep_pat lfin_map_lfset mem_Collect_eq)
      apply (subst Abs_pat_inject)
   apply (metis (mono_tags, lifting) Rep_pat lfin_map_lfset mem_Collect_eq nonrep_prepat_PRec
-      nonrep_prepat_tvsubst_prepat nonrep_prepat_alt)
+      nonrep_prepat_tvsubst_prepat)
   apply (smt (verit, best) Abs_pat_inverse Rep_pat lfin_map_lfset lfset.map_cong_id
-      mem_Collect_eq nonrep_prepat_PRec nonrep_prepat_tvsubst_prepat nonrep_prepat_alt)
+      mem_Collect_eq nonrep_prepat_PRec nonrep_prepat_tvsubst_prepat)
      apply (auto simp: lfset.map_comp intro!: lfset.map_cong) []
   apply (smt (z3) Abs_pat_inverse Rep_pat lfin_map_lfset mem_Collect_eq nonrep_PPRec_def
       nonrep_prepat_PRec nonrep_prepat_tvsubst_prepat
-      tvsubst_prepat.simps(2) nonrep_prepat_alt)
+      tvsubst_prepat.simps(2))
   done
 
 lemma PVars_PVar[simp]: "PVars (PVar x T) = {x}"
-  by (auto simp: PVars_def PVar_def Abs_pat_inverse nonrep_prepat_alt)
+  by (auto simp: PVars_def PVar_def Abs_pat_inverse)
 lemma PVars_PRec[simp]: "nonrep_PRec P \<Longrightarrow> PVars (PRec P) = (\<Union>x \<in> values P. PVars x)"
-  thm Rep_pat[simplified, unfolded nonrep_prepat_alt]
   apply (auto simp: PVars_def PRec_def Abs_pat_inverse nonrep_PRec_alt lfin_map_lfset lfset.set_map Rep_pat[simplified])
-   apply (subst (asm) Abs_pat_inverse[unfolded nonrep_prepat_alt]; auto simp: lfin_map_lfset Rep_pat[simplified, unfolded nonrep_prepat_alt] lfset.set_map)
-   apply (subst Abs_pat_inverse[unfolded nonrep_prepat_alt]; auto simp: lfin_map_lfset Rep_pat[simplified, unfolded nonrep_prepat_alt] lfset.set_map)
+   apply (subst (asm) Abs_pat_inverse; auto simp: lfin_map_lfset Rep_pat[simplified] lfset.set_map)
+   apply (subst Abs_pat_inverse; auto simp: lfin_map_lfset Rep_pat[simplified] lfset.set_map)
   done
-
 lemma PTVars_PVar[simp]: "PTVars (PVar x T) = FVars_typ T"
-  by (auto simp: PTVars_def PVar_def Abs_pat_inverse nonrep_prepat_alt)
+  by (auto simp: PTVars_def PVar_def Abs_pat_inverse)
 lemma PTVars_PRec[simp]: "nonrep_PRec P \<Longrightarrow> PTVars (PRec P) = (\<Union>x \<in> values P. PTVars x)"
   apply (auto simp: PTVars_def PRec_def Abs_pat_inverse nonrep_PRec_alt lfin_map_lfset lfset.set_map Rep_pat[simplified])
-   apply (subst (asm) Abs_pat_inverse[unfolded nonrep_prepat_alt]; auto simp: lfin_map_lfset Rep_pat[simplified, unfolded nonrep_prepat_alt] lfset.set_map)
-   apply (subst Abs_pat_inverse[unfolded nonrep_prepat_alt]; auto simp: lfin_map_lfset Rep_pat[simplified, unfolded nonrep_prepat_alt] lfset.set_map)
+   apply (subst (asm) Abs_pat_inverse; auto simp: lfin_map_lfset Rep_pat[simplified] lfset.set_map)
+   apply (subst Abs_pat_inverse; auto simp: lfin_map_lfset Rep_pat[simplified] lfset.set_map)
   done
 
 lemma finite_PVars[simp]: "finite (PVars P)"
